Completed spy

spy.dfy
@@ -1,6 +1,27 @@
+//recursively choosing pairs according to the given nat
 function method unpair(n: nat): (nat, nat)
 {
-    // Add an implementation for this
+  if n == 0 then
+    (0,0)
+  else
+    var (x,y) := unpair(n-1);
+    if y != 0 then
+      (x+1, y-1)
+    else
+      (y, x+1)
+}
+
+// Show that unpair is correctly choosing pairs
+function unpairCorrect(x: nat, y: nat): nat
+  ensures unpair(unpairCorrect(x,y)) == (x,y)
+  decreases x+y, x
+{
+  if x == 0 && y == 0 then
+    0
+  else if x > 0 then
+    unpairCorrect(x-1, y+1) + 1
+  else
+    unpairCorrect(y-1, 0) + 1
 }
 
 function method pick(i: nat): nat
@@ -14,5 +35,7 @@ method catchTheSpy(a: nat, b: nat)
 var t := 0;
   // prove that this loop terminates and therefore the spy is caught
   while a + t * b != pick(t)
+      invariant t <= unpairCorrect(a, b)
+      decreases unpairCorrect(a,b) - t // Termination
     { t := t + 1; }
 }
